CoqCode/Automations.v
@@ -1,16 +1,3 @@
 Require Import Metalib.Metatheory.
 Require Import Coq.Program.Equality.
-Require Import Language Subtyping Auxiliaries Notations.
-
-Lemma trm_top_checked_by_toplike :
-  forall (A : typ),
-    toplike A ->
-    typing nil nil check_mode trm_top A.
-Proof.
-  intros.
-  eapply typing_sub; eauto.
-  eapply toplike_sub_top. assumption.
-Qed.
-
-Hint Resolve trm_top_checked_by_toplike : core.
-    
+Require Import Language Subtyping Auxiliaries Notations.    
